Strictness for expressions

src/State.v
@@ -11,7 +11,7 @@ From hahn Require Import HahnBase.
 Section S.
 
   Variable A : Set.
-
+  
   Definition state := list (id * A). 
 
   Reserved Notation "st / x => y" (at level 0).
@@ -24,13 +24,57 @@ Section S.
   Definition update (st : state) (id : id) (a : A) : state := (id, a) :: st.
 
   Notation "st [ x '<-' y ]" := (update st x y) (at level 0).
+  
+  Fixpoint st_eval (st : state) (x : id) : option A :=
+    match st with
+    | (x', a) :: st' =>
+        if id_eq_dec x' x then Some a else st_eval st' x
+    | [] => None
+    end.
 
-  Lemma state_deterministic (st : state) (x : id) (n m : A)
-        (SN : st / x => n)
-        (SM : st / x => m) :
+  Lemma state_deterministic' (st : state) (x : id) (n m : option A)
+    (SN : st_eval st x = n)
+    (SM : st_eval st x = m) :
     n = m.
-  Proof. admit. Admitted.
+  Proof using Type.
+    subst n. subst m. reflexivity.
+  Qed.
     
+  Lemma state_deterministic (st : state) (x : id) (n m : A)   
+    (SN : st / x => n)
+    (SM : st / x => m) :
+    n = m. 
+  Proof. admit. Admitted.
+  
+  Lemma eval_binds_eq (st : state) (x : id) :
+      (forall n, st_binds st x n <-> st_eval st x = Some n) /\
+      ((forall n, ~ (st_binds st x n)) <-> st_eval st x = None).
+  Proof.
+    split; split.
+    + intro H. induction H; simpl.
+      - destruct (id_eq_dec id id); [reflexivity | contradiction].
+      - destruct (id_eq_dec id' id); [
+          subst id; contradiction
+        | assumption].
+    + intro H. induction st.
+      - simpl in H. inversion H.
+      - simpl in H. destruct a. destruct (id_eq_dec i x).
+        * subst i. inversion H. constructor.
+        * constructor; auto; unfold not; unfold not in n0; intro; symmetry in H0; auto.
+    + intro H. unfold not in H. induction st.
+      - simpl. reflexivity.
+      - simpl. destruct a. destruct (id_eq_dec i x).
+        * subst i. exfalso. eapply H. constructor.
+        * apply IHst. intros n0 H1. eapply H. constructor. unfold not in n. unfold not. intro. subst x. auto. eassumption.
+    + intro H. induction st.
+      - intro. unfold not. intro. inversion H0.
+      - simpl in H. destruct a. destruct (id_eq_dec i x).
+        * inversion H.
+        * intro. unfold not. intro. unfold not in IHst. eapply IHst.
+          assumption.
+          inversion H0. subst i. subst id. contradiction. eassumption.
+  Qed.
+  
   Lemma update_eq (st : state) (x : id) (n : A) :
     st [x <- n] / x => n.
   Proof. admit. Admitted.
@@ -56,3 +100,6 @@ Section S.
   Proof. admit. Admitted.
 
 End S.
+
+
+Print update_permute.
